Annotated let-statements

LogicalRefinement/Untyped/Subst.lean
@@ -142,7 +142,8 @@ def Term.subst: Term -> Subst -> Term
   | var v, σ => σ v
   | const c, σ => const c
   | unary k t, σ => unary k (t.subst σ)
-  | let_bin k e e', σ => let_bin k (e.subst σ) (e'.subst (σ.liftn 2))
+  | let_bin k P e e', σ => 
+    let_bin k (P.subst σ) (e.subst σ) (e'.subst (σ.liftn 2))
   | bin k l r, σ => bin k (l.subst σ) (r.subst σ)
   | abs k A t, σ => abs k (A.subst σ) (t.subst σ.lift)
   | tri k A l r, σ => tri k (A.subst σ) (l.subst σ) (r.subst σ)
@@ -193,12 +194,12 @@ theorem Term.liftn_wk {u: Term}: {σ: Subst} -> (n: Nat) ->
       intros σ n
       simp only [wknth] at I
       simp only [wknth, wk, subst, I]
-    | let_bin k e e' I I' =>
+    | let_bin k P e e' IP Ie Ie' =>
       intros σ n
       simp only [wknth, wk, subst, Wk.liftn_wknth_merge]
       rw [Subst.liftn_merge]
       simp only [wknth] at *
-      rw [I, I']
+      rw [IP, Ie, Ie']
       simp
     | bin k l r Il Ir =>
       intros σ n
@@ -362,12 +363,14 @@ theorem Term.subst_bounds:
     intros σ n m Hv Hσ;
     simp only [fv, subst];
     exact I Hv Hσ
-  | let_bin k e e' I I' =>
+  | let_bin k P e e' IP Ie Ie' =>
     simp only [fv, subst, Nat.max_r_le_split, Nat.le_sub_is_le_add]
-    intro σ n m ⟨He, He'⟩ Hσ;
+    intro σ n m ⟨HP, He, He'⟩ Hσ;
     apply And.intro
-    exact I He Hσ
-    exact I' He' (Subst.liftn_subst Hσ)
+    exact IP HP Hσ
+    apply And.intro
+    exact Ie He Hσ
+    exact Ie' He' (Subst.liftn_subst Hσ)
   | bin k l r Il Ir =>
     intros σ n m;
     simp only [Term.fv, Nat.max_r_le_split]
